riscv_model/code/mod32_lemmas.dfy
@@ -1,0 +1,63 @@
+include "../spec/rsa_ops.dfy"
+
+module mod32_lemmas {
+  
+    import opened bv_ops
+    import opened rv_ops
+    import opened rsa_ops
+    import opened rv_consts
+    import opened powers
+    import opened congruences
+
+    const B  : int := BASE_32;
+    const B2 : int := B * B;
+
+    function sub_mod32_update_A(A:int, a:int, n:int) : int64 
+    {
+      to_int64(A + a - n)
+    }
+
+    predicate sub_mod32_loop_inv(
+      iter_a: iter_t,
+      iter_n: iter_t,
+      iter_a': iter_t,
+      A: int64)
+    {
+      && (A == 0 || A == -1)
+      && var i := iter_a.index;
+      && |iter_a.buff| == |iter_n.buff| == |iter_a'.buff|
+      && (i == iter_a'.index == iter_n.index)
+      && i <= |iter_a.buff|
+      && seq_subb(iter_a.buff[..i], iter_n.buff[..i]) == (iter_a'.buff[..i], neg1_to_uint1(A))
+    }
+
+    lemma lemma_sub_mod32_correct(
+      A: int64_view_t, // old A
+      A': int64_view_t, // new A
+      iter_a: iter_t,
+      iter_n: iter_t,
+      iter_a': iter_t,
+      iter_a_next: iter_t,
+      iter_n_next: iter_t,
+      iter_a'_next: iter_t,
+      x15: uint32,
+      x13: uint32)
+      requires
+        && sub_mod32_loop_inv(iter_a, iter_n, iter_a', A)
+        && iter_a.index < |iter_a.buff| // still in bounds after increment
+        && x15 == uint32_add(iter_a.buff[i], A.lh)
+        && x13 == uint32_sub(x15, iter_n.buff[i])
+        && carry_add == uint32_lt(x15, iter_a.buff[i])
+        && carry_sub == uint32_lt(x15, x13)
+        && A.uh + carry_add
+        && iter_a_next == lw_iter_next(iter_a)
+        && iter_n_next == lw_iter_next(iter_n)
+        && iter_a'_next == sw_iter_next(iter_a', x13)
+      ensures
+        sub_mod32_loop_inv(lw_iter_next(iter_a), lw_iter_next(iter_n), iter_a', A');
+
+      {
+        assume false;
+      }
+
+}
